code/experimental/P256/Hacl.Impl.ECDSA.P256SHA256.Signature.fst
@@ -14,7 +14,7 @@ open Hacl.Spec.P256.Lemmas
 open Hacl.Spec.ECDSAP256.Definition
 open Hacl.Impl.LowLevel
 open Hacl.Spec.P256.Basic
-open Hacl.Spec.P256.Core
+
 
 open Hacl.Impl.ECDSA.MontgomeryMultiplication
 open Hacl.Impl.ECDSA.MM.Exponent
