code/experimental/P256/Hacl.Impl.P256.fst
@@ -8,8 +8,6 @@ open Lib.IntTypes
 open Lib.IntTypes.Compatibility
 open Lib.Buffer
 
-open Hacl.Spec.P256.Core
-
 open Hacl.Spec.P256.Lemmas
 open Hacl.Spec.P256.Definitions
 open Hacl.Impl.SolinasReduction
