code/experimental/P256/Hacl.Impl.SolinasReduction.fst
@@ -12,7 +12,7 @@ open Lib.Buffer
 open Hacl.Spec.P256.SolinasReduction
 open Hacl.Impl.LowLevel
 open Hacl.Impl.P256.LowLevel
-open Hacl.Spec.P256.Core
+
 open Hacl.Spec.P256.Definitions
 open FStar.Mul
 
