code/experimental/P256/Hacl.Impl.SolinasReduction.fsti
@@ -11,7 +11,7 @@ open Lib.Buffer
 
 open Hacl.Spec.P256.SolinasReduction
 open Hacl.Impl.LowLevel
-open Hacl.Spec.P256.Core
+
 open Hacl.Spec.P256.Definitions
 open FStar.Mul
 
