code/experimental/P256/Hacl.Spec.P256.MontgomeryMultiplication.PointAdd.fst
@@ -5,9 +5,9 @@ open FStar.Math.Lemmas
 open FStar.Math.Lib
 open Hacl.Spec.P256.Lemmas
 open Hacl.Spec.P256.Definitions
-open Hacl.Spec.P256.Core
+
 open Lib.Sequence
-open Hacl.Spec.P256.Core
+
 open Hacl.Spec.P256.MontgomeryMultiplication
 open Lib.Loops
 open FStar.Mul
